incr with some assumes

ulib/experimental/Steel.Swap.fst
@@ -9,51 +9,116 @@ open Steel.SteelT.Basics
 
 
 
-// let reference (a:Type0) = reference a (fun _ _ -> True)
-// let writable = full_permission
-// let pts_to_ref (#a:Type0) (r:reference a) (p:permission{allows_read p}) (x:a) = pts_to_ref r p x
-// let ref_perm (#a:Type0) (r:reference a) = ref_perm r
+let reference (a:Type0) = reference a (fun _ _ -> True)
+let writable = full_permission
+let pts_to_ref (#a:Type0) (r:reference a) (p:permission{allows_read p}) (x:a) = pts_to_ref r p x
+let ref_perm (#a:Type0) (r:reference a) = ref_perm r
 
-// let sel_ref (#a:Type0) (r:reference a) (m:hmem (ref r)) = sel_ref r m
+let sel_ref (#a:Type0)
+  (r:reference a) (p:permission{allows_read p}) (m:hmem (ref_perm r p)) =
+  assume (forall (m:mem). interp (ref_perm r p) m ==> interp (ref r) m);
+  sel_ref r m
 
-// assume val weaken_pts_to_ref (#a:Type0) (r:reference a) (p:permission{allows_read p}) (x:a)
+assume val sel_ref_depends_only_on (#a:Type0) (r:reference a) (p:permission{allows_read p}) (m0:mem) (m1:mem)
+: Lemma
+  (requires
+    interp (ref_perm r p) m0 /\
+    disjoint m0 m1)
+  (ensures
+    interp (ref_perm r p) (join m0 m1) /\
+    sel_ref r p m0 == sel_ref r p (join m0 m1))
+  [SMTPat (sel_ref r p (join m0 m1))]
+
+assume val read (#a:Type0) (#p:permission{allows_read p}) (r:reference a)
+: Steel a
+    (ref_perm r p)
+    (fun _ -> ref_perm r p)
+    (fun _ -> True) (fun m0 x m1 -> sel_ref r p m0 == x /\ sel_ref r p m1 == x)
+
+assume val write (#a:Type0) (r:reference a) (x:a)
+: Steel unit
+    (ref_perm r writable)
+    (fun _ -> ref_perm r writable)
+    (fun _ -> True)
+    (fun _ _ m -> sel_ref r writable m == x)
+
+let incr (r:reference int)
+: Steel unit
+    (ref_perm r writable)
+    (fun _ -> ref_perm r writable)
+    (fun _ -> True)
+    (fun m0 _ m1 -> sel_ref r writable m1 == sel_ref r writable m0 + 1)
+= let x = read r in
+  write r (x+1)
+
+
+
+// assume val sel_ref_core (#a:Type0) (r:reference a) (p:permission{allows_read p}) (m:mem)
 // : Lemma
-//   (forall (m:mem). interp (pts_to_ref r p x) m ==> interp (ref_perm r p) m)
-//   [SMTPat (pts_to_ref r p x)]
+//   (requires interp (ref_perm r p) m)
+//   (ensures sel_ref r p m == sel_ref r p (core_mem m))
+//   [SMTPat (sel_ref r p (core_mem m))]
 
-// assume val weaken_ref_perm (#a:Type0) (r:reference a) (p:permission{allows_read p})
+// assume Interp_depends_only_on:
+//   forall (hp:hprop) (m0:hmem hp) (m1:mem{disjoint m0 m1}).
+//      interp hp m0 == interp hp (join m0 m1)
+
+// assume val core_mem_interp (hp:hprop) (m:mem)
 // : Lemma
-//   (forall (m:mem). interp (ref_perm r p) m ==> interp (ref r) m)
-//   [SMTPat (ref_perm r p)]
+//   (interp hp (core_mem m) == interp hp m)
+//   [SMTPat (interp hp (core_mem m))]
 
-// assume val sel_ref_depends_only_on (#a:Type0) (r:reference a) (m0:mem) (m1:mem)
+
+
+// let sel_ref_is_a_refinement (#a:Type0) (r:reference a) (x:a)
 // : Lemma
-//   (requires
-//     interp (ref r) m0 /\
-//     disjoint m0 m1)
-//   (ensures
-//     interp (ref r) (join m0 m1) /\
-//     sel_ref r m0 == sel_ref r (join m0 m1))
-//   [SMTPat (sel_ref r (join m0 m1))]
+//   (forall (m0:hmem (ref r)) (m1:mem{disjoint m0 m1}).
+//      (interp (ref r) m0 /\ sel_ref r m0 == x)  <==>
+//      (interp (ref r) (join m0 m1) /\ sel_ref r (join m0 m1) == x))
+// = ()
 
-// assume val sel_ref_core (#a:Type0) (r:reference a) (m:mem)
+
+// let sel_ref_is_a_refinement (#a:Type0) (r:reference a) (x:a)
 // : Lemma
-//   (requires interp (ref r) m)
-//   (ensures sel_ref r m == sel_ref r (core_mem m))
-//   [SMTPat (sel_ref r (core_mem m))]
+//   (forall m0 m1. ((interp (ref r) m0 /\ sel_ref r m0 == x) /\ disjoint m0 m1) ==>
+//             (interp (ref r) (join m0 m1) /\ sel_ref r (join m0 m1) == x))
+// = ()
 
-// assume val read (#a:Type0) (#p:permission{allows_read p}) (r:reference a) (_:unit)
-// : Steel a
-//     (ref_perm r p)
-//     (fun x -> pts_to_ref r p x)
-//     (fun _ -> True) (fun _ x m -> sel_ref r m == x)
 
-// assume val write (#a:Type0) (r:reference a) (x:a) (_:unit)
-// : Steel unit
-//     (ref_perm r writable)
-//     (fun _ -> pts_to_ref r writable x)
-//     (fun _ -> True)
-//     (fun _ _ m -> sel_ref r m == x)
+// let sel_ref_is_a_refinement (#a:Type0) (r1:reference a)
+// : Lemma
+//   (forall m x. (interp (ref r1) m /\ sel_ref r1 m == x) == (interp (ref r1) (core_mem m) /\ sel_ref r1 (core_mem m) == x))
+// = ()
+
+// unfold
+// let sel_ref_mprop (#a:Type0) (r:reference a) (p:permission{allows_read p}) (x:a)
+// : mem -> prop
+// = fun m -> interp (ref_perm r p) m /\ sel_ref r p m == x
+
+// #push-options "--warn_error -271"
+// let sel_ref_depends_only_on_aux (#a:Type0) (r:reference a) (p:permission{allows_read p}) (x:a)
+// : Lemma
+//   (forall (m:mem). (interp (ref_perm r p) m /\ sel_ref r p m == x) == (interp (ref_perm r p) (core_mem m) /\ sel_ref r p (core_mem m) == x))
+// = let aux (m:mem)
+//     : Lemma
+//       ((interp (ref_perm r p) m /\ sel_ref r p m == x) == (interp (ref_perm r p) (core_mem m) /\ sel_ref r p (core_mem m) == x))
+//       [SMTPat ()]
+//     = FStar.PropositionalExtensionality.apply (sel_ref_mprop r p x m) (sel_ref_mprop r p x (core_mem m)) in
+//   ()
+// #pop-options
+
+// let sel_ref_refine_depends_only_on (#a:Type0) (r:reference a) (p:permission{allows_read p}) (x:a)
+// : Lemma
+//   (sel_ref_mprop r p x `refine_mprop_depends_only_on` (ref_perm r p))
+// = sel_ref_depends_only_on_aux r p x
+
+
+// unfold
+// let sel_ref_as_refinement (#a:Type0) (r:reference a) (p:permission{allows_read p}) (x:a)
+// : refine_mprop (ref_perm r p)
+// = sel_ref_refine_depends_only_on r p x;
+//   sel_ref_mprop r p x
+
 
 // assume val refine_intro (p0 p1:hprop) (q:refine_mprop p0)
 // : Steel unit
@@ -71,62 +136,7 @@ open Steel.SteelT.Basics
 // assume val steel_admit (#a:_) (#pre:pre_t) (#post:post_t a) (_:unit)
 // : Steel a pre post (fun _ -> True) (fun _ _ _ -> False)
 
-// // assume Interp_depends_only_on:
-// //   forall (hp:hprop) (m0:hmem hp) (m1:mem{disjoint m0 m1}).
-// //      interp hp m0 == interp hp (join m0 m1)
 
-// assume val core_mem_interp (hp:hprop) (m:mem)
-// : Lemma
-//   (interp hp (core_mem m) == interp hp m)
-//   [SMTPat (interp hp (core_mem m))]
-
-// // let sel_ref_is_a_refinement (#a:Type0) (r:reference a) (x:a)
-// // : Lemma
-// //   (forall (m0:hmem (ref r)) (m1:mem{disjoint m0 m1}).
-// //      (interp (ref r) m0 /\ sel_ref r m0 == x)  <==>
-// //      (interp (ref r) (join m0 m1) /\ sel_ref r (join m0 m1) == x))
-// // = ()
-
-
-// // let sel_ref_is_a_refinement (#a:Type0) (r:reference a) (x:a)
-// // : Lemma
-// //   (forall m0 m1. ((interp (ref r) m0 /\ sel_ref r m0 == x) /\ disjoint m0 m1) ==>
-// //             (interp (ref r) (join m0 m1) /\ sel_ref r (join m0 m1) == x))
-// // = ()
-
-
-// // let sel_ref_is_a_refinement (#a:Type0) (r1:reference a)
-// // : Lemma
-// //   (forall m x. (interp (ref r1) m /\ sel_ref r1 m == x) == (interp (ref r1) (core_mem m) /\ sel_ref r1 (core_mem m) == x))
-// // = ()
-
-// unfold
-// let sel_ref_mprop (#a:Type0) (r:reference a) (x:a)
-// : mem -> prop
-// = fun m -> interp (ref r) m /\ sel_ref r m == x
-
-// #push-options "--warn_error -271"
-// let sel_ref_depends_only_on_aux (#a:Type0) (r:reference a) (x:a)
-// : Lemma
-//   (forall (m:mem). (interp (ref r) m /\ sel_ref r m == x) == (interp (ref r) (core_mem m) /\ sel_ref r (core_mem m) == x))
-// = let aux (m:mem)
-//     : Lemma
-//       ((interp (ref r) m /\ sel_ref r m == x) == (interp (ref r) (core_mem m) /\ sel_ref r (core_mem m) == x))
-//       [SMTPat ()]
-//     = FStar.PropositionalExtensionality.apply (sel_ref_mprop r x m) (sel_ref_mprop r x (core_mem m)) in
-//   ()
-// #pop-options
-
-// let sel_ref_refine_depends_only_on (#a:Type0) (r:reference a) (x:a)
-// : Lemma
-//   (sel_ref_mprop r x `refine_mprop_depends_only_on` (ref r))
-// = sel_ref_depends_only_on_aux r x
-
-// unfold
-// let sel_ref_as_refinement (#a:Type0) (r:reference a) (x:a)
-// : refine_mprop (ref r)
-// = sel_ref_refine_depends_only_on r x;
-//   sel_ref_mprop r x
 
 // let swap (#a:Type0) (r1 r2:reference a)
 // : Steel unit
@@ -163,7 +173,3 @@ open Steel.SteelT.Basics
 
 //   steel_admit ()
 
-  
-  
-//   steel_admit ()
- 
